finished ceval_step_ceval

software-foundation-8.5/ImpCEvalFun.v
@@ -68,6 +68,96 @@ Fixpoint ceval_step3 (st : state) (c : com) (i : nat) : option state :=
   end.
 
 
+Notation "'LETOPT' x <== e1 'IN' e2"
+  := (match e1 with
+      | Some x => e2
+      | None => None
+      end)
+       (right associativity, at level 60).
+
+
         
       
+
+Fixpoint ceval_step (st : state) (c : com) (i : nat)
+                    : option state :=
+  match i with
+  | O => None
+  | S i' =>
+      match c with
+      | SKIP =>
+             Some st
+      | l ::= a1 =>
+          Some (t_update st l (aeval st a1))
+      | c1 ;; c2 =>
+           LETOPT st' <== ceval_step st c1 i' IN
+           ceval_step st' c2 i'
+      | IFB b THEN c1 ELSE c2 FI =>
+            if (beval st b)
+            then ceval_step st c1 i'
+            else ceval_step st c2 i'
+      | WHILE b1 DO c1 END =>
+              if (beval st b1)
+              then LETOPT st' <== ceval_step st c1 i' IN
+                          ceval_step st' c i'
+              else Some st
+      end
+  end.
+
+Definition test_ceval (st:state) (c:com) :=
+  match ceval_step st c 500 with
+  | None => None
+  | Some st => Some (st X, st Y, st Z)
+  end.
+
+
+
+Definition pup_to_n : com :=
+  Y ::= ANum 0;;
+    WHILE BNot (BEq (AId X) (ANum 0)) DO
+          Y ::= APlus (AId Y) (AId X);;
+    X ::= AMinus (AId X) (ANum 1)
+      END.
+
+Example pup_to_n_1 :
+  test_ceval (t_update empty_state X 5) pup_to_n
+  = Some (0, 15, 0).
+Proof. reflexivity. Qed.
+
+Definition peven : com :=
+  Z ::= AId X;;
+    WHILE BNot (BLe (AId Z) (ANum 1)) DO
+        Z ::= AMinus (AId Z) (ANum 2)
+    END.
+
+
+Theorem ceval_step_ceval : forall c st st',
+    (exists i, ceval_step st c i = Some st') ->
+    c / st \\ st'.
+Proof.
+  intros c st st' [i E].
+  generalize dependent st'.
+  generalize dependent st.
+  generalize dependent c.
+  induction i.
+  intros c st st' H. inversion H.
+  intros c st st' H.
+  destruct c; simpl in H; inversion H; subst; clear H.
+  apply E_Skip.
+  apply E_Ass. auto.
+  destruct (ceval_step st c1 i) eqn:Heqr.
+  apply E_Seq with s. apply IHi. assumption.
+  apply IHi. assumption. inversion H1.
+  destruct (beval st b) eqn: Heqr.
+  apply E_IfTrue. auto. apply IHi. assumption.
+  apply E_IfFalse. auto. apply IHi. assumption.
+  destruct (beval st b) eqn: Heqr.
+  destruct (ceval_step st c i) eqn:Heqr1.
+  apply E_WhileLoop with s. auto.
+  apply IHi. auto.
+  apply IHi. auto.
+  inversion H1.
+  inversion H1.
+  apply E_WhileEnd. subst. auto.
+Qed.
 
